Skip to content

Latest commit

 

History

History
278 lines (211 loc) · 10.8 KB

shape_4_impl_2.rst

File metadata and controls

278 lines (211 loc) · 10.8 KB

Shape class 4, impl=2

This implementation of Shape 4 <shape_4> is designed for exploiting symmetric spatial resolutions.


Δkx = Δky,  nx = ny

For short, we will apply the notation Δk = Δkx = Δky and n = nx = ny. It follows that


Y − jy(y) = jy(y),  Z − jy, jx(z) = Zjy, jx(z),  Zjx, jy(z) = Zjy, jx(z)

where jy(y) denotes the complex conjugate of Yjy(y). Consequently, we apply the following equivalent wave field formulation.

$$\phi(x,y,z,t) = \sum_{j_x=0}^{n}\sum_{j_y=0}^{j_x} \mathcal{Re} \Bigl\{C_{j_y,j_x}(x, y, t)\Bigr\}\, Z_{j_y,j_x}(z)$$

$$\zeta(x,y,t) = \sum_{j_x=0}^{n}\sum_{j_y=0}^{j_x} \mathcal{Re} \Bigl\{H_{ j_y,j_x}(x, y, t)\Bigr\}$$

$$\begin{aligned} C_{j_y,j_x}(x, y, t) = &\bigl( c_{1,j_y,j_x}(t)\,Y_{j_y}(y) + c_{2,j_y,j_x}(t)\, \bar{Y}_{j_y}(y)\bigr) X_{j_x}(x) +\\\ &\bigl( c_{3,j_y,j_x}(t)\,Y_{j_x}(y) + c_{4,j_y,j_x}(t)\, \bar{Y}_{j_x}(y)\bigr) X_{j_y}(x) \end{aligned}$$

$$\begin{aligned} H_{j_y,j_x}(x, y, t) = &\bigl( h_{1,j_y,j_x}(t)\,Y_{j_y}(y) + h_{2,j_y,j_x}(t)\, \bar{Y}_{j_y}(y)\bigr) X_{j_x}(x) +\\\ &\bigl( h_{3,j_y,j_x}(t)\,Y_{j_x}(y) + h_{4,j_y,j_x}(t)\, \bar{Y}_{j_x}(y)\bigr) X_{j_y}(x) \end{aligned}$$

$$\begin{aligned} c_{1,j_y,j_x}(t) = c_{j_y,j_x}(t), \qquad c_{2,j_y,j_x}(t) = \begin{cases} c_{-j_y,j_x}(t), & \text{$j_y>0$}, \\\ 0, & \text{$j_y=0$} \end{cases} \\\ c_{3,j_y,j_x}(t) = \begin{cases} c_{j_x,j_y}(t), & \text{$j_y<j_x$}, \\\ 0, & \text{$j_y=j_x$} \end{cases}, \qquad c_{4,j_y,j_x}(t) = \begin{cases} c_{-j_x,j_y}(t), & \text{$j_y<j_x$}, \\\ 0, & \text{$j_y=j_x$} \end{cases} \\\ h_{1,j_y,j_x}(t) = h_{j_y,j_x}(t), \qquad h_{2,j_y,j_x}(t) = \begin{cases} h_{-j_y,j_x}(t), & \text{$j_y>0$}, \\\ 0, & \text{$j_y=0$} \end{cases} \\\ h_{3,j_y,j_x}(t) = \begin{cases} h_{j_x,j_y}(t), & \text{$j_y<j_x$}, \\\ 0, & \text{$j_y=j_x$} \end{cases}, \qquad h_{4,j_y,j_x}(t) = \begin{cases} h_{-j_x,j_y}(t), & \text{$j_y<j_x$}, \\\ 0, & \text{$j_y=j_x$} \end{cases} \end{aligned}$$

$$k_{j_x} = j_x\cdot\Delta k, \quad k_{j_y} = j_y\cdot\Delta k, \quad k_{j_y,j_x} = \sqrt{j_x^2+ j_y^2}\, \Delta k, \quad i = \sqrt{-1}$$

Kinematics

Given the definitions above we obtain the following explicit kinematics:

$$\phi(\bar{x},\bar{y},\bar{z},\bar{t})= \sum_{j_x=0}^{n}\sum_{j_y=0}^{j_x} \mathcal{Re} \Bigl\{C_{j_y,j_x}(x, y, t)\Bigr\} Z_{j_y,j_x}(z)$$


φ(, , , ) ≡ 0

$$\frac{\partial\phi}{\partial \bar{t}}(\bar{x},\bar{y},\bar{z},\bar{t}) = \sum_{j_x=0}^{n}\sum_{j_y=0}^{j_x} \mathcal{Re} \Bigl\{\frac{d C_{j_y,j_x}(x, y, t)}{dt}\Bigr\} Z_{j_y,j_x}(z)$$

$$\zeta(\bar{x},\bar{y},\bar{t})= \sum_{j_x=0}^{n}\sum_{j_y=0}^{j_x} \mathcal{Re}\Bigl\{H_{j_y,j_x}(x, y, t)\Bigr\}$$

$$\frac{\partial\zeta}{\partial \bar{t}}(\bar{x},\bar{y},\bar{t}) = \sum_{j_x=0}^{n}\sum_{j_y=0}^{j_x} \mathcal{Re} \Bigl\{\frac{d H_{j_y,j_x}(x, y, t)}{dt}\Bigr\}$$

$$\frac{\partial\zeta}{\partial \bar{x}}(\bar{x},\bar{y},\bar{t}) = \zeta_x\cos\beta - \zeta_y\sin\beta, \qquad \frac{\partial\zeta}{\partial \bar{y}}(\bar{x},\bar{y},\bar{t}) = \zeta_x\sin\beta + \zeta_y\cos\beta$$

$$\zeta_x =\sum_{j_x=0}^{n}\sum_{j_y=0}^{j_x} \mathcal{Im} \Bigl\{H_{j_y,j_x}^{1,0}(x, y, t)\Bigr\}$$

$$\zeta_y = \sum_{j_x=0}^{n}\sum_{j_y=0}^{j_x} \mathcal{Im} \Bigl\{H_{j_y,j_x}^{0,1}(x, y, t)\Bigr\}$$

$$\bar{\nabla}\phi(\bar{x},\bar{y},\bar{z},\bar{t}) = [\phi_x\cos\beta - \phi_y\sin\beta, \phi_x\sin\beta + \phi_y\cos\beta,\phi_z]^T$$

$$\phi_x = \sum_{j_x=0}^{n}\sum_{j_y=0}^{j_x} \mathcal{Im} \Bigl\{C_{j_y,j_x}^{1,0}(x, y, t)\Bigr\} \, Z_{j_y,j_x}(z)$$

$$\phi_y = \sum_{j_x=0}^{n}\sum_{j_y=0}^{j_x} \mathcal{Im} \Bigl\{C_{j_y,j_x}^{0,1}(x, y, t)\Bigr\} \, Z_{j_y,j_x}(z)$$

$$\phi_z = \sum_{j_x=0}^{n}\sum_{j_y=0}^{j_x} k_{j_y,j_x} \mathcal{Re} \Bigl\{C_{j_y,j_x}(x, y, t)\Bigr\} \, Z_{j_y,j_x}(z)$$

$$\frac{\partial\bar{\nabla}\phi}{\partial \bar{t}}(\bar{x},\bar{y},\bar{z},\bar{t}) = [\phi_{xt}\cos\beta - \phi_{yt}\sin\beta, \phi_{xt}\sin\beta + \phi_{yt}\cos\beta,\phi_z]^T$$

$$\phi_{xt} = \sum_{j_x=0}^{n}\sum_{j_y=0}^{j_x} \mathcal{Im} \Bigl\{\frac{d C_{j_y,j_x}^{1,0}(x, y, t)}{dt}\Bigr\} \, Z_{j_y,j_x}(z)$$

$$\phi_{yt} = \sum_{j_x=0}^{n}\sum_{j_y=0}^{j_x} \mathcal{Im} \Bigl\{\frac{d C_{j_y,j_x}^{0,1}(x, y, t)}{dt}\Bigr\} \, Z_{j_y,j_x}(z)$$

$$\phi_{zt} = \sum_{j_x=0}^{n}\sum_{j_y=0}^{j_x} k_{j_y,j_x} \mathcal{Re} \Bigl\{\frac{d C_{j_y,j_x}(x, y, t)}{dt}\Bigr\} \, Z_{j_y,j_x}(z)$$

$$\frac{d\bar{\nabla}\phi}{d\bar{t}}(\bar{x},\bar{y},\bar{z},\bar{t}) = \frac{\partial\bar{\nabla}\phi}{\partial \bar{t}} + \bar{\nabla}\phi \cdot \bar{\nabla}\bar{\nabla}\phi$$

$$\begin{aligned} \bar{\nabla}\bar{\nabla}\phi (\bar{x},\bar{y},\bar{z},\bar{t}) = \begin{bmatrix} \phi_{\bar{x},\bar{x}} & \phi_{\bar{x},\bar{y}} & \phi_{\bar{x},\bar{z}} \\\ \phi_{\bar{x},\bar{y}} & \phi_{\bar{y},\bar{y}} & \phi_{\bar{y},\bar{z}} \\\ \phi_{\bar{x},\bar{z}} & \phi_{\bar{y},\bar{z}} & \phi_{\bar{z},\bar{z}} \end{bmatrix} \end{aligned}$$


ϕ,  = ϕxxcos2β − ϕxysin (2β) + ϕyysin2β


ϕ,  = ϕxy(cos2β − sin2β) + (ϕxx − ϕyy)sin βcos β


ϕ,  = ϕxzcos β − ϕyzsin β


ϕ,  = ϕyycos2β + ϕxysin (2β) + ϕxxsin2β


ϕ,  = ϕyzcos β + ϕxzsin β


ϕ,  = ϕzz =  − ϕxx − ϕyy

$$\phi_{xx} = - \sum_{j_x=0}^{n}\sum_{j_y=0}^{j_x} \mathcal{Re} \Bigl\{C_{j_y,j_x}^{2,0}(x, y, t)\Bigr\} Z_{j_y,j_x}(z)$$

$$\phi_{xy} = - \sum_{j_x=0}^{n}\sum_{j_y=0}^{j_x} \mathcal{Re} \Bigl\{C_{j_y,j_x}^{1,1}(x, y, t)\Bigr\} Z_{j_y,j_x}(z)$$

$$\phi_{xz} = \sum_{j_x=0}^{n}\sum_{j_y=0}^{j_x} k_{j_y,j_x} \mathcal{Im} \Bigl\{C_{j_y,j_x}^{1,0}(x, y, t)\Bigr\} Z_{j_y,j_x}(z)$$

$$\phi_{yy} = - \sum_{j_x=0}^{n}\sum_{j_y=0}^{j_x} \mathcal{Re} \Bigl\{C_{j_y,j_x}^{0,2}(x, y, t)\Bigr\} Z_{j_y,j_x}(z)$$

$$\phi_{yz} = \sum_{j_x=0}^{n}\sum_{j_y=0}^{j_x} k_{j_y,j_x} \mathcal{Im} \Bigl\{C_{j_y,j_x}^{0,1}(x, y, t)\Bigr\} Z_{j_y,j_x}(z)$$

$$\phi_{zz} = \sum_{j_x=0}^{n}\sum_{j_y=0}^{j_x} k_{j_y,j_x}^2 \mathcal{Re} \Bigl\{C_{j_y,j_x}(x, y, t)\Bigr\} Z_{j_y,j_x}(z) = -\phi_{xx} - \phi_{yy}$$

$$\frac{\partial^2\zeta}{\partial \bar{x}^2}(\bar{x},\bar{y},\bar{t}) = \zeta_{xx}\cos^2\beta - \zeta_{xy}\sin(2\beta) + \zeta_{yy}\sin^2\beta$$

$$\frac{\partial^2\zeta}{\partial\bar{x}\partial\bar{y}}(\bar{x},\bar{y},\bar{t}) = \zeta_{xy}(\cos^2\beta - \sin^2\beta) + (\zeta_{xx} - \zeta_{yy})\sin\beta\cos\beta$$

$$\frac{\partial^2\zeta}{\partial\bar{y}^2}(\bar{x},\bar{y},\bar{t}) = \zeta_{yy}\cos^2\beta + \zeta_{xy}\sin(2\beta) + \zeta_{xx}\sin^2\beta$$

$$\zeta_{xx} = -\sum_{j_x=0}^{n}\sum_{j_y=0}^{j_x} \mathcal{Re} \Bigl\{H_{j_y,j_x}^{2,0}(x, y, t)\Bigr\}$$

$$\zeta_{xy} = -\sum_{j_x=0}^{n}\sum_{j_y=0}^{j_x} \mathcal{Re} \Bigl\{H_{j_y,j_x}^{1,1}(x, y, t)\Bigr\}$$

$$\zeta_{yy} = -\sum_{j_x=0}^{n}\sum_{j_y=0}^{j_x} \mathcal{Re} \Bigl\{H_{j_y,j_x}^{0,2}(x, y, t)\Bigr\}$$

$$p = -\rho\frac{\partial\phi}{\partial \bar{t}} -\frac{1}{2}\rho\bar{\nabla}\phi\cdot\bar{\nabla}\phi -\rho g \bar{z}$$

where $\bar{\nabla}$ denotes gradients with respect to , and . We also apply the notation

$$\begin{aligned} \frac{\partial^{i+j}C_{j_y,j_x}(x, y, t)}{\partial x^i \partial y^j} = (-i)^{i+j} C_{j_y,j_x}^{i,j}(x, y, t) \\\ \frac{\partial^{i+j}H_{j_y,j_x}(x, y, t)}{\partial x^i \partial y^j} = (-i)^{i+j} H_{j_y,j_x}^{i,j}(x, y, t) \end{aligned}$$

$$\begin{aligned} C_{j_y,j_x}^{i,j}(x, y, t) = &k_{j_x}^ik_{j_y}^j\bigl( c_{1,j_y,j_x}(t)\,Y_{j_y}(y) +(-1)^j c_{2,j_y,j_x}(t)\, \bar{Y}_{j_y}(y)\bigr) X_{j_x}(x) +\\\ &k_{j_y}^i k_{j_x}^j\bigl( c_{3,j_y,j_x}(t)\,Y_{j_x}(y) + (-1)^j c_{4,j_y,j_x}(t)\, \bar{Y}_{j_x}(y)\bigr) X_{j_y}(x) \end{aligned}$$

$$\begin{aligned} H_{j_y,j_x}^{i,j}(x, y, t) = &k_{j_x}^ik_{j_y}^j\bigl( h_{1,j_y,j_x}(t)\,Y_{j_y}(y) +(-1)^j h_{2,j_y,j_x}(t)\, \bar{Y}_{j_y}(y)\bigr) X_{j_x}(x) +\\\ &k_{j_y}^i k_{j_x}^j\bigl( h_{3,j_y,j_x}(t)\,Y_{j_x}(y) + (-1)^j h_{4,j_y,j_x}(t)\, \bar{Y}_{j_x}(y)\bigr) X_{j_y}(x) \end{aligned}$$

The particle acceleration is labeled $\frac{d\bar{\nabla}\phi}{d\bar{t}}$.

The stream function φ is not relevant for short crested seas. Hence, we apply the dummy definition φ = 0 for all locations.

Implementation notes

Evaluation of costly transcendental functions (cos , sin , exp , ...) is significantly reduced by exploiting the following recursive relations


Xjx(x) = X1(x) Xjx − 1(x),  Yjy(y) = Y1(y) Yjy − 1(y)

It should be noted that contrary to long crested seas, there are no trivial recursive relations for the z-dependent term Zjy, jx(z). This makes calculations of surface elevations significantly faster than calculations of other kinematics for short crested seas.

In case the wave generator<wave-generator> applies a perturbation theory of order q we apply the following Taylor expansion above the calm free surface.

$$Z_{j_y, j_x}(z) = 1 + \sum_{p=1}^{q-1}\frac{(k_{j_y, j_x} z)^p}{p!}, \qquad z > 0$$